proxyLatest.bpl
@@ -22,8 +22,8 @@ requires n1 > 0;
 procedure UnpackBasicFieldsRealSum(su:real, n1:int, this:Ref);
 requires packedBasicFieldsRealSum[this];
 requires fracBasicFieldsRealSum[this] > 0.0;
-ensures	(n[this]==n1);
-ensures (sum[this] == su);
+requires (n[this]==n1);
+requires (sum[this] == su);
 ensures n1 > 0;
 
 procedure PackSumOKRealSum(n1:int, this:Ref);
@@ -35,7 +35,7 @@ requires ( sum[this] == (n1 * (n1+1) / 2) );
 procedure UnpackSumOKRealSum(n1:int, this:Ref);
 requires packedSumOKRealSum[this];
 requires fracSumOKRealSum[this] > 0.0;
-ensures	(n[this]==n1);
+requires (n[this]==n1);
 ensures n1 > 0;
 ensures	(sum[this] == (n1 * (n1+1) / 2) );
 
@@ -47,7 +47,7 @@ requires (s1 > 0.0);
 procedure UnpackSumGreater0RealSum(s1:real, this:Ref);
 requires packedSumGreater0RealSum[this];
 requires fracSumGreater0RealSum[this] > 0.0;
-ensures (sum[this] == s1);
+requires (sum[this] == s1);
 ensures	(s1 > 0.0);
 
 procedure ConstructRealSum(n1:int, this:Ref)
@@ -186,9 +186,9 @@ requires (n1 > 0);
 procedure UnpackBasicFieldsProxySum(rs:Ref, su:real, n1:int, this:Ref);
 requires packedBasicFieldsProxySum[this];
 requires fracBasicFieldsProxySum[this] > 0.0;
-ensures (realSum[this] == rs);
-ensures (sum[this] == su);
-ensures	(n[this] == n1);
+requires (realSum[this] == rs);
+requires (sum[this] == su);
+requires (n[this] == n1);
 ensures (n1 > 0);
 
 procedure PackSumOKProxySum(n1:int, this:Ref);
@@ -200,7 +200,7 @@ requires ( sum[this] == n1 * (n1+1) / 2 );
 procedure UnpackSumOKProxySum(n1:int, this:Ref);
 requires packedSumOKProxySum[this];
 requires fracSumOKProxySum[this] > 0.0;
-ensures	(n[this] == n1);
+requires (n[this] == n1);
 ensures n1 > 0;
 ensures (sum[this] == (n1 * (n1+1) / 2));
 
@@ -212,7 +212,7 @@ requires (s1 > 0.0);
 procedure UnpackSumGreater0ProxySum(s1:real, this:Ref);
 requires packedSumGreater0ProxySum[this];
 requires fracSumGreater0ProxySum[this] > 0.0;
-ensures (sum[this] == s1);
+requires (sum[this] == s1);
 ensures	(s1 > 0.0);
 
 procedure ConstructProxySum(n1:int, this:Ref)
@@ -346,7 +346,7 @@ requires (instanceof[suCli] == 2) ==> (fracSumOKRealSum[suCli] > 0.0) ;
 procedure UnpackClientSumOK(suCli:Ref, this:Ref);
 requires packedClientSumOK[this];
 requires fracClientSumOK[this] > 0.0;
-ensures sumClient[this] == suCli;
+requires sumClient[this] == suCli;
 // TODO add requires about parameters if needed
 ensures (instanceof[suCli] == 1) ==> (fracSumOKProxySum[suCli] > 0.0) ;
 ensures (instanceof[suCli] == 2) ==> (fracSumOKRealSum[suCli] > 0.0) ;
@@ -361,7 +361,7 @@ requires (instanceof[suCli] == 2) ==> (fracSumGreater0RealSum[suCli] > 0.0) ;
 procedure UnpackClientSumGreater0(suCli:Ref, this:Ref);
 requires packedClientSumGreater0[this];
 requires fracClientSumGreater0[this] > 0.0;
-ensures sumClient[this] == suCli;
+requires sumClient[this] == suCli;
 // TODO add requires about parameters if needed
 ensures (instanceof[suCli] == 1) ==> (fracSumGreater0ProxySum[suCli] > 0.0) ;
 ensures (instanceof[suCli] == 2) ==> (fracSumGreater0RealSum[suCli] > 0.0) ;
